dafny/src/util/bond.dfy
@@ -1,55 +1,176 @@
-include "../util/number.dfy"
-include "../util/maps.dfy"
-include "../util/tx.dfy"
+
+include "number.dfy"
+include "maps.dfy"
+include "tx.dfy"
+include "fixed.dfy"
 include "../erc20.dfy"
 
 
 import opened Number
 import opened Maps
 import opened Tx
+import opened Fixed
 
 
-class Bond {
-  // a 160-bit unsigned integer that uniquely identifies the address. However,
-  // this value is not directly used as the external representation, that is in u256
-    var usdc: ERC20
-    var bond: ERC20
+class LendingProtocol {
+    var totalBorrow: u256
+    var totalReserve: u256
+    var totalDeposit: u256
+    const maxLTV: u256 := 4
+    var ethTreasury: u256
+    var totalCollateral: u256
+    const baseRate: u256 := 20000000000000000
+    const fixedAnnuBorrowRate: u256 := 300000000000000000
 
-    const baseRate: u256 := 20_000_000_000_000_000    // 0.02 [wad]
-    const annuRate: u256 := 300_000_000_000_000_000   // 0.3  [wad]
+    var usersCollateral: mapping<u160, u256>  // ETH
+    var usersBorrowed: mapping<u160, u256>    // DAI
+    var usersBalances: mapping<u160, u256>    // DAI
 
-    // totals
-    var borrow:  u256
-    var lends:   u256
-    var reserve: u256
-    var collateral: u256
-    var balances:   mapping<u160, u256>
-    var user_collateral: mapping<u160, u256>
-    var borrowed:   mapping<u160, u256>
+    const WAD: u256 := 1000000000000000000
+    const HALF_WAD: u256 := WAD / 2
+
+    var DAI: ERC20
+    var bDAI: ERC20
 
     constructor() {
-        usdc := new ERC20();
-        bond := new ERC20();
-        borrow    := 0;
-        lends     := 0;
-        collateral:= 0;
+        usersCollateral := Map(map[], 0);
+        usersBorrowed := Map(map[], 0);
+        usersBalances := Map(map[], 0);
+
+        DAI := new ERC20();
+        bDAI := new ERC20();
     }
 
-    // supply collateral for lending
-    method supply(msg: Transaction, amount: u256) returns (r: Result<()>)
-    modifies this`collateral
-    requires amount as nat <= MAX_U256 - collateral.Get(msg.sender) as nat {
-        collateral := balances.Set(msg.sender, collateral.Get(msg.sender) + amount);
+    method bondAsset(msg: Transaction, amount: u256)
+    modifies this`totalDeposit
+    requires this.totalDeposit as nat + amount as nat <= MAX_U256 as nat {
+        // usersBalances := 
+        totalDeposit := totalDeposit + amount;
+    }
+    
+
+    method addCollateral(msg: Transaction, amount: u256) returns (r: Result<()>)
+    modifies this`usersCollateral
+    requires amount as nat <= MAX_U256 - usersCollateral.Get(msg.sender) as nat {
+        usersCollateral := usersBalances.Set(msg.sender, usersCollateral.Get(msg.sender) + amount);
         return Ok(());
     }
 
-
-    method remove(msg: Transaction, amount: u256) returns (r: Result<()>)
-    modifies this`collateral
-    requires amount as nat <= collateral.Get(msg.sender) as nat {
-        collateral := balances.Set(msg.sender, collateral.Get(msg.sender) - amount);
+    method removeCollateral(msg: Transaction, amount: u256) returns (r: Result<()>)
+    modifies this`usersCollateral
+    requires amount as nat <= usersCollateral.Get(msg.sender) as nat {
+        usersCollateral := usersBalances.Set(msg.sender, usersCollateral.Get(msg.sender) - amount);
         return Ok(());
     }
+
+    method getExp(x: u256, y: u256) returns (result: u256)
+    requires x as nat * WAD as nat <= MAX_U256 as nat
+    requires y != 0
+    {
+        var mul: u256 := Mul(x, WAD);
+        result := Fixed.Div(mul, y);
+    }
+ 
+
+    method mulExp(x: u256, y: u256) returns (result: u256)
+    requires x as nat * y as nat <= MAX_U256 as nat
+    {
+        var mul: u256 := Mul(x, y);
+        assume {:axiom} (HALF_WAD as nat) + (mul as nat) <= MAX_U256 as nat;
+        var add: u256 := Add(HALF_WAD, mul);
+        result := Fixed.Div(add, WAD);
+    }
+
+    method utilizationRatio() returns (utilizationRatio: u256)
+    requires this.totalBorrow as nat * WAD as nat <= MAX_U256 as nat
+    requires this.totalDeposit != 0
+    {
+        utilizationRatio := getExp(this.totalBorrow, this.totalDeposit);
+    }
+
+    method interestMultiplier() returns (interestMul: u256)
+    requires this.fixedAnnuBorrowRate > this.baseRate
+    requires this.totalBorrow as nat * WAD as nat <= MAX_U256 as nat
+    requires this.totalDeposit != 0
+    {
+        var uRatio: u256 := utilizationRatio();
+        var num: u256 := Sub(this.fixedAnnuBorrowRate, this.baseRate);
+        assume {:axiom} (uRatio as nat) > 0 as nat;
+        interestMul := getExp(num, uRatio);
+    }
+    
+
+    method borrowRate() returns (rate: u256)
+    requires this.fixedAnnuBorrowRate > this.baseRate
+    requires this.totalBorrow as nat * WAD as nat <= MAX_U256 as nat
+    requires this.totalDeposit != 0
+    {
+        var uRatio: u256 := utilizationRatio();
+        var interestMul: u256 := interestMultiplier();
+        assume {:axiom} (uRatio as nat) * (interestMul as nat) <= MAX_U256 as nat;
+        var product := mulExp(uRatio, interestMul);
+        assume {:axiom} (product as nat) + (baseRate as nat) <= MAX_U256 as nat;
+        rate := Add(product, baseRate);
+    }
+
+    // method calculateBorrowFee(amount: u256) returns (fee: u256, paid: u256)
+    method calculateBorrowFee(amount: u256) returns (paid: u256)
+    requires this.totalBorrow as nat * WAD as nat <= MAX_U256 as nat
+    requires this.totalDeposit != 0
+    {
+        var borrowRate: u256 := borrowRate();
+        assume {:axiom} (amount as nat) * (borrowRate as nat) <= MAX_U256 as nat;
+        var fee: u256 := Mul(amount, borrowRate);
+        assume {:axiom} (amount as nat) - (fee as nat) >= 0 as nat;
+        paid := Sub(amount, fee);
+    }
+}
+
+
+// --- TESTS
+
+import opened Fixed
+import opened Number
+import opened Maps
+import opened Tx
+
+method {:test} testLendingProtocol() {
+    // Instantiate the LendingProtocol class
+    var protocol := new LendingProtocol();
+
+    // Set necessary values for totalDeposit and totalBorrow using setter methods
+    protocol.totalDeposit := 100; // Setting totalDeposit to 1 ether (for example)
+    protocol.totalBorrow := 100;   // Setting totalBorrow to 0.5 ether (for example)
+
+    // protocol.totalDeposit := 100;
+
+    assert protocol.totalDeposit == 100;
+    assert protocol.totalBorrow == 100;
+
+    // Define the amount for which the borrow fee needs to be calculated
+    var borrowAmount: u256 := 20; // Example borrow amount
+
+    // Declare variables to store the results
+    var fee: u256;
+    var paid: u256;
+
+    // Call the calculateBorrowFee method and store the results
+    paid := protocol.calculateBorrowFee(borrowAmount);
+
+    //assert paid == 14;
+
+    // Print or assert the results to verify correctness
+    // print "Borrow Fee: ", fee, "\n";
+    // print "Amount Paid: ", paid, "\n";
+
+    // Optionally, you can include assertions to check expected values
+    // assert fee >= 0;
+    // assert paid == borrowAmount - fee;
+
+    var a: u256 := WAD;
+    var b : u256 :=WAD;
+    var c : u256 := protocol.getExp(a , b );
+    assert c < WAD;
 
 
 
