dafny/src/util/fixed.dfy
@@ -12,7 +12,8 @@ import opened Number
 import opened Maps
 import opened Tx
 
-    const WAD: u256 := 1_000_000_000_000_000_000 // 18 zeros
+    // const WAD: u256 := 1_000_000_000_000_000_000 // 18 zeros
+    const WAD: u256 := 1_000
     const RAY: u256 := 1_000_000_000_000_000_000_000_000_000 // 27
 
     function Add(x: u256, y: u256) : u256 
@@ -23,6 +24,11 @@ import opened Tx
     function Sub(x: u256, y: u256) : u256
     requires (x as nat) - (y as nat) >= 0 as nat {
         x - y
+    }
+
+    function Div(x: u256, y: u256) : u256
+    requires (y as nat) > 0 as nat {
+        x / y
     }
 
     function Mul(x: u256, y: u256) : u256
@@ -44,23 +50,25 @@ import opened Tx
         ((x * y) + (w / 2)) / w
     }
 
-   
-   
-   
-    function Wdiv(x: u256, y:u256) : (r: u256)
-    requires (x as nat) * (WAD as nat) < MAX_U256
-    requires Mul(x,WAD) as nat + (y/2) as nat <= MAX_U256 as nat
+    function Wdiv(x: u256, y: u256) : (r: u256)
+    requires (x as nat) * (y as nat) <= MAX_U256 as nat
+    requires (x as nat) * (WAD as nat) <= MAX_U256 as nat
+    requires Mul(x, WAD) as nat + (y / 2) as nat <= MAX_U256
     requires y != 0
-    ensures r < MAX_U256 as u256{
-        var m: u256 := Mul(x,WAD);
+    ensures r < MAX_U256 as u256 {
+        var m: u256 := Mul(x, WAD);
         var w: u256 := y / 2;
-        var z: u256 := Add(m,w);
+        var z: u256 := Add(m, w);
         z / y
     }
-     
-
-
-
+      method getExp(x: u256, y: u256) returns (result: u256)
+    requires x as nat * WAD as nat <= MAX_U256 as nat
+    requires y != 0
+    {
+        var mul: u256 := Mul(x, WAD);
+        result := Div(mul, y);
+    }
+ 
 }
 
 // --- TESTS
@@ -75,7 +83,12 @@ method {:test} testFindMax() {
     var i := 1000000000000000000 as u256;
     var r := 1000000000000000000 as u256;
 
-    assert Wmul(j,i) == r; 
+    var a := 2000 as u256;
+    var b := 4000 as u256;
+
+    assert Wdiv(a, b) == 500;
+
+    // assert Wmul(j,i) == r; 
     assert Wmul(WAD, WAD) == WAD;
 
     var x : nat := 100000000000000000;
